feat(core): add guarded PTree interpreters

theories/Core/PTreeDefinitionNew.v
@@ -157,6 +157,25 @@ Definition trigger {E M} : E ~> ptree E M :=
   fun _ e => Vis e (fun x => Ret x).
 Arguments trigger {E M T} _.
 
+(** Interpret visible events with a PTree handler.  The administrative
+    [Tau] on the visible branch makes the corecursion syntactically guarded;
+    it is intentionally invisible to the canonical weak equivalence. *)
+Definition interp {E F M} (handler : E ~> ptree F M) {R}
+    (t : ptree E M R) : ptree F M R :=
+  (cofix interp_ (u : ptree E M R) : ptree F M R :=
+    match observe u with
+    | RetF r => Ret r
+    | TauF u' => Tau (interp_ u')
+    | @VisF _ _ _ _ X e k =>
+        Tau (bind (handler _ e) (fun x => interp_ (k x)))
+    | @ProbF _ _ _ _ X mu k => Prob mu (fun x => interp_ (k x))
+    end) t.
+
+(** Event renaming is the pure-handler instance of [interp]. *)
+Definition translate {E F M} (f : E ~> F) {R}
+    (t : ptree E M R) : ptree F M R :=
+  interp (fun _ e => @trigger F M _ (f _ e)) t.
+
 End PTree.
 
 
